Finish verification of fib exaple programs
This includes the delay version and the state_delay version of fib.
Both are verified both as a top level definition using just the nth
number. But through helper lemmas that can start at any step, this is to
make the induction work.

The key to verifying both is the coq_fib_move' Lemma that let's us move
the addition out of the post condition from the iterative version into
the recursive version.

Remember to not simpl too much in wp_state_delay definitions since it
breaks the abstraction layer.

theories/program_logic/delay_examples.v
@@ -1,4 +1,3 @@
-
 From iris.proofmode Require Import base tactics classes.
 From iris.base_logic.lib Require Export fancy_updates.
 From shiris.program_logic Require Import delaystate.
@@ -44,9 +43,11 @@ Qed.
 Section state_ad.
 Context `{! inG Σ (heapR natO)}.
 
-Lemma post' (n1 n2 n: nat) (ret: nat): iProp Σ.
+Definition post' (n1 n2 n: nat) (ret: nat): iProp Σ.
 refine( ⌜ret = coq_fib n1 n2 n⌝%I).
 Defined.
+
+Definition post (n ret: nat): iProp Σ := post' 0 1 n ret.
 
 Lemma coq_fib_unfold n1 n2 n: 
     coq_fib n1 n2 (S (S n)) = coq_fib n1 n2 (S n) + coq_fib n1 n2 n.
@@ -99,43 +100,64 @@ Lemma coq_fib_move' n1 n2 n:
 Lemma verify_delay_fib' n1 n2 n:
     ⊢ wp_delay (delaystate.iter fib' (n, n1, n2)) (post' n1 n2 n).
 Proof.
-    (*How do i vary the IH here properly *)
     iLöb as "IH" forall (n n1 n2).
     iApply wp_delay_iter. 
-    destruct n as [| n'] eqn: E .
+    destruct n as [| n'] eqn: E.
     - iApply wp_delay_return. done.
     - iApply wp_delay_return. simpl. 
       iNext.
       iApply (wp_strong_mono_delay with "IH").
-      unfold post'.
-      iIntros (v Hv) "!%".
-      subst v.
+      iIntros (v Hv) "!%". subst v.
       apply coq_fib_move'.
 Qed.
 
 Lemma verify_delay_fib n:
-    True -∗ wp_delay (fib n) (post n).
+    ⊢ wp_delay (fib n) (post n).
 Proof.
-
-Definition iter_adder (l k: nat): () -> state_delay (gmap nat nat) (() + nat) :=
-  λ _, x  ← get l ;
-       y  ← get k ; 
-       if x =? 0 then mret $ inr y 
-       else put l (x - 1) ;; put k (y + 1) ;; mret $ inl () .
+    unfold fib. unfold post.
+    apply (@verify_delay_fib' 0 1 n).
+Qed.
 
 Definition fib_state' (l1 l2: nat) (n: nat): state_delay (gmap nat nat) (nat + nat) :=
     match n with
     | S n' => n1 ← get l1 ;
               n2 ← get l2 ;
-              put l1 n1 ;; put l2 (n1 + n2) ;; mret $ inl n'
-    | O => inr <$> get l2
+              put l1 n2 ;; put l2 (n1 + n2) ;; mret $ inl n'
+    | O => inr <$> get l1
     end.
 
-Definition fib_state (l1 l2 n: nat): state_delay (gmap nat nat) nat := 
+Lemma verify_delay_state_fib' l1 l2 n1 n2 n:
+    ∀ γ, points_to γ l1 n1 ∗ points_to γ l2 n2 -∗
+            wp (state_interp γ) (iter_state_delay (fib_state' l1 l2) n) (post' n1 n2 n).
+Proof.
+    iIntros (γ) "(Hl1 & Hl2)".
+    iLöb as "IH" forall (n n1 n2).
+    iApply wp_iter.
+    destruct n as [| n'] eqn: E.
+    - iApply wp_fmap. iApply (wp_get with "Hl1").
+      iIntros "Hl1". done.
+    -
+     iApply wp_bind. iApply (wp_get with "Hl1"). iIntros "Hl1".
+     iApply wp_bind. iApply (wp_get with "Hl2"). iIntros "Hl2".
+     iApply wp_bind. iApply (wp_put with "Hl1"). iIntros "Hl1".
+     iApply wp_bind. iApply (wp_put with "Hl2"). iIntros "Hl2".
+     iApply wp_return. 
+     iNext. 
+     iSpecialize ("IH" with "Hl1 Hl2").
+     iApply (wp_strong_mono with "IH").
+     iIntros (v Hv) "!%". subst v.
+     apply coq_fib_move'.
+Qed.
+
+Definition fib_state (n: nat): state_delay (gmap nat nat) nat := 
+    l1 ← alloc 0 ;
+    l2 ← alloc 1 ;
     iter_state_delay (fib_state' l1 l2) n.
 
-Lemma verify_delay_state_fib l1 l2 n:
-    ∀ γ, points_to γ l1 1 ∗ points_to γ l2 1 -∗
-            wp (state_interp γ) (fib_state l1 l2 n) (λ ret, ⌜ret = coq_fib 0 1 n⌝).
+Lemma verify_delay_state_fib γ n:
+     ⊢ wp (state_interp γ) (fib_state n) (post n).
 Proof.
-Admitted.
+    iApply wp_bind. iApply wp_alloc. iIntros (l1) "Hl1".
+    iApply wp_bind. iApply wp_alloc. iIntros (l2) "Hl2".
+    iApply verify_delay_state_fib'. iFrame.
+Qed.
